Intermediate/PS.v
@@ -3,9 +3,9 @@ Require Import Common.Util.
 Require Import Common.Events.
 Require Import Common.Smallstep.
 Require Import Intermediate.Machine.
-Require Import Intermediate.CPS.
+Require Import Intermediate.CS.
 
-Module PPS.
+Module PS.
   Import IntermediateMachine.
 
   Record program := {
@@ -46,7 +46,7 @@ Module PPS.
       if Util.mem C pc then (C, Some i) else (C, None)
     end.
 
-  Definition to_partial_stack (s : CPS.stack) (pc : list Component.id) :=
+  Definition to_partial_stack (s : CS.stack) (pc : list Component.id) :=
     map (to_partial_frame pc) s.
 
   Lemma push_by_prog_preserves_partial_stack :
@@ -110,10 +110,10 @@ Module PPS.
 
   Definition maps_match_on {T : Type} split (map map' : M.t T) :=
     forall C Cmap,
-      PPS.is_program_component C split ->
+      PS.is_program_component C split ->
       (M.MapsTo C Cmap map <-> M.MapsTo C Cmap map').
 
-  Reserved Notation "G |-PPS s1 '=>[' t ']' s2" (at level 40).
+  Reserved Notation "G |-PS s1 '=>[' t ']' s2" (at level 40).
 
   Inductive step (G : global_env)
     : partial_state -> trace -> partial_state -> Prop :=
@@ -124,11 +124,11 @@ Module PPS.
         M.MapsTo C cmem wmem ->
         M.MapsTo C cmem' wmem' ->
         maps_match_on (genv_split G) E (genv_entrypoints G) ->
-        let G' := CPS.mkGlobalEnv (genv_interfaces G) E in
-        CPS.step G' (C,s,wmem,regs,pc) E0 (C,s,wmem',regs',pc') ->
+        let G' := CS.mkGlobalEnv (genv_interfaces G) E in
+        CS.step G' (C,s,wmem,regs,pc) E0 (C,s,wmem',regs',pc') ->
         M.MapsTo C cmem mem ->
         M.MapsTo C cmem' mem' ->
-        G |-PPS (PC (C,ps,mem,regs,pc)) =>[E0] (PC (C,ps,mem',regs',pc'))
+        G |-PS (PC (C,ps,mem,regs,pc)) =>[E0] (PC (C,ps,mem',regs',pc'))
 
   | Program_Internal_Call:
       forall mem C pc regs d d' C' P,
@@ -139,7 +139,7 @@ Module PPS.
         is_program_component C' (genv_split G) ->
         d' = (C,Some (pc+1)) :: d ->
         let t := [ECall C P (Register.get Register.R_COM regs) C'] in
-        G |-PPS (PC (C,d,mem,regs,pc)) =>[t]
+        G |-PS (PC (C,d,mem,regs,pc)) =>[t]
                 (PC (C',d',mem,regs,EntryPoint.get C' P (genv_entrypoints G)))
 
   | Program_Internal_Return:
@@ -149,7 +149,7 @@ Module PPS.
         is_program_component C' (genv_split G) ->
         d = (C',Some pc') :: d' ->
         let t := [ERet C (Register.get Register.R_COM regs) C'] in
-        G |-PPS (PC (C,d,mem,regs,pc)) =>[t] (PC (C',d',mem,regs,pc'))
+        G |-PS (PC (C,d,mem,regs,pc)) =>[t] (PC (C',d',mem,regs,pc'))
 
   | Program_External_Call:
       forall mem C pc regs d d' C' P,
@@ -160,7 +160,7 @@ Module PPS.
         is_context_component C' (genv_split G) ->
         d' = (C,Some (pc+1)) :: d ->
         let t := [ECall C P (Register.get Register.R_COM regs) C'] in
-        G |-PPS (PC (C,d,mem,regs,pc)) =>[t] (CC (C',d',mem) Normal)
+        G |-PS (PC (C,d,mem,regs,pc)) =>[t] (CC (C',d',mem) Normal)
 
   | Program_External_Return:
       forall mem C C' pc d d' regs,
@@ -169,15 +169,15 @@ Module PPS.
         is_context_component C' (genv_split G) ->
         d = (C',None) :: d' ->
         let t := [ERet C (Register.get Register.R_COM regs) C'] in
-        G |-PPS (PC (C,d,mem,regs,pc)) =>[t] (CC (C',d',mem) Normal)
+        G |-PS (PC (C,d,mem,regs,pc)) =>[t] (CC (C',d',mem) Normal)
 
   | Context_Epsilon:
       forall mem C d,
-        G |-PPS (CC (C,d,mem) Normal) =>[E0] (CC (C,d,mem) Normal)
+        G |-PS (CC (C,d,mem) Normal) =>[E0] (CC (C,d,mem) Normal)
 
   | Context_GoesWrong:
       forall mem C d,
-        G |-PPS (CC (C,d,mem) Normal) =>[E0] (CC (C,d,mem) WentWrong)
+        G |-PS (CC (C,d,mem) Normal) =>[E0] (CC (C,d,mem) WentWrong)
 
   | Context_Internal_Call:
       forall mem C d d' C' P call_arg,
@@ -187,7 +187,7 @@ Module PPS.
         is_context_component C' (genv_split G) ->
         d' = (C,None) :: d ->
         let t := [ECall C P call_arg C'] in
-        G |-PPS (CC (C,d,mem) Normal) =>[t] (CC (C',d',mem) Normal)
+        G |-PS (CC (C,d,mem) Normal) =>[t] (CC (C',d',mem) Normal)
 
   | Context_Internal_Return:
       forall mem C C' d d' return_val,
@@ -195,7 +195,7 @@ Module PPS.
         is_context_component C' (genv_split G) ->
         d = (C',None) :: d' ->
         let t := [ERet C return_val C'] in
-        G |-PPS (CC (C,d,mem) Normal) =>[t] (CC (C',d',mem) Normal)
+        G |-PS (CC (C,d,mem) Normal) =>[t] (CC (C',d',mem) Normal)
 
   | Context_External_Call:
       forall mem C regs d d' C' P,
@@ -205,7 +205,7 @@ Module PPS.
         is_program_component C' (genv_split G) ->
         d' = (C,None) :: d ->
         let t := [ECall C P (Register.get Register.R_COM regs) C'] in
-        G |-PPS (CC (C,d,mem) Normal) =>[t]
+        G |-PS (CC (C,d,mem) Normal) =>[t]
                 (PC (C',d',mem,regs,EntryPoint.get C' P (genv_entrypoints G)))
 
   | Context_External_Return:
@@ -213,9 +213,9 @@ Module PPS.
         d = (C',Some pc') :: d' ->
         is_program_component C' (genv_split G) ->
         let t := [ERet C (Register.get Register.R_COM regs) C'] in
-        G |-PPS (CC (C,d,mem) Normal) =>[t] (PC (C',d',mem,regs,pc'))
+        G |-PS (CC (C,d,mem) Normal) =>[t] (PC (C',d',mem,regs,pc'))
 
-  where "G |-PPS s1 '=>[' t ']' s2" := (step G s1 t s2).
+  where "G |-PS s1 '=>[' t ']' s2" := (step G s1 t s2).
 
   Lemma maps_match_on_reflexive :
     forall T split (map : M.t T),
@@ -237,81 +237,84 @@ Module PPS.
   Hint Resolve maps_match_on_symmetric.
 
   Lemma update_related_memories_generic :
-    forall split mem1 mem2 C Cmem C' addr val,
+    forall split mem1 mem1' mem2 mem2' C Cmem C' addr val,
       maps_match_on split mem1 mem2 ->
       is_program_component C split ->
-      M.MapsTo C Cmem (Memory.set mem1 C' addr val) ->
-      M.MapsTo C Cmem (Memory.set mem2 C' addr val).
+      Some mem1' = Memory.set mem1 C' addr val ->
+      Some mem2' = Memory.set mem2 C' addr val ->
+      M.MapsTo C Cmem mem1' ->
+      M.MapsTo C Cmem mem2'.
   Proof.
-    intros split mem1 mem2 C Cmem C' addr val.
-    intros Hmems_match HCorigin HCmem.
+    intros split mem1 mem1' mem2 mem2' C Cmem C' addr val.
+    intros Hmems_match HCorigin Hmem1upd Hmem2upd HCmem.
     unfold Memory.set.
     unfold Memory.set in HCmem.
     destruct (C =? C') eqn:HeqCC'.
     + apply beq_nat_true in HeqCC'. subst.
-      destruct (M.find (elt:=list nat) C' mem2) eqn:Hfind.
-      * apply M.find_2 in Hfind. apply Hmems_match in Hfind.
-        ** rewrite (M.find_1 Hfind) in HCmem.
-           apply M.find_2.
-           apply M.find_1 in HCmem.
-           rewrite <- HCmem.
-           rewrite F.add_eq_o, F.add_eq_o;
-             reflexivity.
-        ** assumption.
-      * apply Hmems_match.
-        ** assumption.
-        ** assert (M.find (elt:=list nat) C' mem1 = None).
-           { destruct (M.find (elt:=list nat) C' mem1) eqn:Hfind'.
-             *** exfalso.
-                 apply F.not_find_in_iff in Hfind. apply Hfind.
-                 exists l. apply Hmems_match.
-                 **** assumption.
-                 **** apply M.find_2. assumption.
-             *** reflexivity. }
-           rewrite H in HCmem. assumption.
+      unfold Memory.set in Hmem1upd, Hmem2upd.
+      destruct (M.find (elt:=list nat) C' mem1) eqn:Hfind_mem1.
+      * destruct (M.find (elt:=list nat) C' mem2) eqn:Hfind_mem2.
+        ** inversion Hmem1upd as [Hmem1]. inversion Hmem2upd as [Hmem2].
+           subst. rewrite (CS.MapsTo_extraction _ _ _ _ HCmem).
+           enough (l = l0). subst.
+           apply M.add_1; auto.
+           apply F.find_mapsto_iff in Hfind_mem1.
+           apply F.find_mapsto_iff in Hfind_mem2.
+           apply Hmems_match in Hfind_mem1.
+           apply (F.MapsTo_fun Hfind_mem1 Hfind_mem2); auto.
+           auto.
+        ** inversion Hmem2upd.
+      * inversion Hmem1upd.
     + apply beq_nat_false in HeqCC'.
-      destruct (M.find (elt:=list nat) C' mem2) eqn:Hfind.
-      * apply M.add_2.
-        ** unfold not. intro. apply HeqCC'. symmetry. apply H.
-        ** apply Hmems_match.
-           *** assumption.
-           *** destruct (M.find (elt:=list nat) C' mem1) eqn:Hfind'.
-               **** eapply M.add_3.
-                    ***** intro. apply HeqCC'. symmetry. apply H.
-                    ***** apply HCmem.
+      unfold Memory.set in Hmem1upd, Hmem2upd.
+      destruct (M.find (elt:=list nat) C' mem1) eqn:Hfind_mem1.
+      * destruct (M.find (elt:=list nat) C' mem2) eqn:Hfind_mem2.
+        ** inversion Hmem1upd as [Hmem1]. inversion Hmem2upd as [Hmem2].
+           subst. apply M.add_2.
+           *** unfold not. intro. apply HeqCC'. symmetry. apply H.
+           *** apply Hmems_match.
                **** assumption.
-      * apply Hmems_match.
-        ** assumption.
-        ** destruct (M.find (elt:=list nat) C' mem1) eqn:Hfind'.
-           *** eapply M.add_3.
-               **** intro. apply HeqCC'. symmetry. apply H.
-               **** apply HCmem.
-           *** assumption.
+               **** destruct (M.find (elt:=list nat) C' mem1) eqn:Hfind'.
+                    ***** eapply M.add_3.
+                    ****** intro. apply HeqCC'. symmetry. apply H.
+                    ****** apply HCmem.
+                    ***** inversion Hfind_mem1.
+        ** inversion Hmem2upd.
+      * inversion Hmem1upd.
   Qed.
 
   Lemma update_related_memories :
     forall split mem1 mem1' mem2 mem2' C addr val,
       maps_match_on split mem1 mem2 ->
-      mem1' = Memory.set mem1 C addr val ->
-      mem2' = Memory.set mem2 C addr val ->
+      Some mem1' = Memory.set mem1 C addr val ->
+      Some mem2' = Memory.set mem2 C addr val ->
       maps_match_on split mem1' mem2'.
   Proof.
     intros split mem1 mem1' mem2 mem2' C addr val.
-    intros Hmems_match Hmem1' Hmem2'.
-    unfold PPS.maps_match_on.
+    intros Hmems_match Hmem1'_ Hmem2'_.
+    unfold PS.maps_match_on.
     intros C0 C0mem HC0_origin.
-    split;
-      intro HC0map;
-      [ rewrite Hmem2';
-        rewrite Hmem1' in HC0map;
-        apply update_related_memories_generic with
-            (split:=split) (mem1:=mem1) (mem2:=mem2)
-      | rewrite Hmem1';
-        rewrite Hmem2' in HC0map;
-        apply update_related_memories_generic with
-            (split:=split) (mem1:=mem2) (mem2:=mem1) ];
-      auto.
-  Qed.
+    destruct (C =? C0) eqn:HCC0.
+    - rewrite beq_nat_true_iff in HCC0. subst. auto.
+      split.
+      apply update_related_memories_generic with
+          (mem1:=mem1) (mem2:=mem2) (C':=C0)
+          (split:=split) (addr:=addr) (val:=val);
+        auto.
+      apply update_related_memories_generic with
+          (mem1:=mem2) (mem2:=mem1) (C':=C0)
+          (split:=split) (addr:=addr) (val:=val);
+        auto.
+    - split.
+      apply update_related_memories_generic with
+          (mem1:=mem1) (mem2:=mem2) (C':=C)
+          (split:=split) (addr:=addr) (val:=val);
+        auto.
+      apply update_related_memories_generic with
+          (mem1:=mem2) (mem2:=mem1) (C':=C)
+          (split:=split) (addr:=addr) (val:=val);
+        auto.
+  Qed.  
 
   Section SEMANTICS.
     Variable p : program.
@@ -331,23 +334,23 @@ Module PPS.
      to the components in the split *)
   Lemma entrypoints_exist_wrt_split split :
     forall p CI C,
-      In CI (CPS.prog_interface p) ->
+      In CI (CS.prog_interface p) ->
       Component.name CI = C ->
       In C split ->
-      M.In C (CPS.prog_entrypoints p) /\
-      exists addrs, M.MapsTo C addrs (CPS.prog_entrypoints p).
+      M.In C (CS.prog_entrypoints p) /\
+      exists addrs, M.MapsTo C addrs (CS.prog_entrypoints p).
   Proof.
     intros p CI C.
     intros HCI_in_I HCI_name_is_C HC_in_split.
-    apply (CPS.prog_entrypoints_wf p) with CI; assumption.
+    apply (CS.prog_entrypoints_wf p) with CI; assumption.
   Qed.
 
-  Definition apply_split (p : CPS.program) split splitWF :=
-    {| prog_interface := CPS.prog_interface p;
-       prog_memory := CPS.prog_memory p;
-       prog_entrypoints := CPS.prog_entrypoints p;
+  Definition apply_split (p : CS.program) split splitWF :=
+    {| prog_interface := CS.prog_interface p;
+       prog_memory := CS.prog_memory p;
+       prog_entrypoints := CS.prog_entrypoints p;
        prog_split := split;
        prog_entrypoints_wf :=
          entrypoints_exist_wrt_split split p;
        prog_split_wf := splitWF |}.
-End PPS.
+End PS.
